reorganize(Sepref) pull stuff from hnr_primitives to the front

thys/sepref/Hnr_Primitives_Experiment.thy
@@ -1,65 +1,10 @@
 theory Hnr_Primitives_Experiment
-imports Sepref_Basic "../ds/LLVM_DS_Dflt"
+imports Sepref_Rules "../ds/LLVM_DS_Dflt"
 begin
   hide_const (open) LLVM_DS_Array.array_assn
 
-  subsubsection \<open>Composition\<close>
-  definition hr_comp :: "('b \<Rightarrow> 'c \<Rightarrow> assn) \<Rightarrow> ('b \<times> 'a) set \<Rightarrow> 'a \<Rightarrow> 'c \<Rightarrow> assn"
-    \<comment> \<open>Compose refinement assertion with refinement relation\<close>
-    where "hr_comp R1 R2 a c \<equiv> EXS b. R1 b c ** \<up>((b,a)\<in>R2)"
-
-  lemma hr_compI: "(b,a)\<in>R2 \<Longrightarrow> R1 b c \<turnstile> hr_comp R1 R2 a c"  
-    unfolding hr_comp_def
-    by (auto simp: sep_algebra_simps entails_def pred_lift_extract_simps)
-
-  lemma hr_comp_Id1[simp]: "hr_comp (pure Id) R = pure R"  
-    unfolding hr_comp_def[abs_def] pure_def
-    apply (intro ext)
-    by (auto simp: pred_lift_extract_simps)
-
-  lemma hr_comp_Id2[simp]: "hr_comp R Id = R"  
-    unfolding hr_comp_def[abs_def]
-    apply (intro ext)
-    by (auto simp: sep_algebra_simps pred_lift_extract_simps)
-    
-  lemma hr_comp_emp[simp]: "hr_comp (\<lambda>a c. \<box>) R a c = \<up>(\<exists>b. (b,a)\<in>R)"
-    unfolding hr_comp_def[abs_def]
-    apply (intro ext)
-    by (auto simp: sep_algebra_simps pred_lift_extract_simps)
-
-  lemma hr_comp_prod_conv[simp]:
-    "hr_comp (prod_assn Ra Rb) (Ra' \<times>\<^sub>r Rb') 
-    = prod_assn (hr_comp Ra Ra') (hr_comp Rb Rb')"  
-    unfolding hr_comp_def[abs_def] prod_assn_def[abs_def]
-    apply (intro ext)
-    apply (auto 0 3 simp: sep_algebra_simps pred_lift_extract_simps)
-    done
-
-  lemma hr_comp_pure: "hr_comp (pure R) S = pure (R O S)"  
-    apply (intro ext)
-    unfolding hr_comp_def[abs_def] pure_def
-    by (auto simp: sep_algebra_simps pred_lift_extract_simps)
-
-  lemma hr_comp_is_pure: "is_pure A \<Longrightarrow> is_pure (hr_comp A B)"
-    by (auto simp: hr_comp_pure is_pure_conv)
-
-  lemma hr_comp_the_pure: "is_pure A \<Longrightarrow> the_pure (hr_comp A B) = the_pure A O B"
-    unfolding is_pure_conv
-    by (clarsimp simp: hr_comp_pure)
-
-  lemma rdomp_hrcomp_conv[simp]: "rdomp (hr_comp A R) x \<longleftrightarrow> (\<exists>y. rdomp A y \<and> (y,x)\<in>R)"
-    by (auto simp: rdomp_def hr_comp_def sep_algebra_simps pred_lift_extract_simps)
-
-  lemma hr_comp_assoc: "hr_comp (hr_comp R S) T = hr_comp R (S O T)"
-    apply (intro ext)
-    unfolding hr_comp_def
-    by (auto simp: sep_algebra_simps pred_lift_extract_simps)
-
-
-lemma conc_fun_spec_ne_FAIL[simp]: "\<Down>R (SPECT M) \<noteq> FAILT" by (simp add: conc_fun_RES)   
-    
-(*lemma project_acost_conc_fun[refine_pw_simps]: "project_acost b (\<Down>R m) = \<Down>R (project_acost b m)" sorry*)
-
+experiment
+begin
 
 lemma aux_abs_help:
   fixes M :: "_ \<rightharpoonup> ecost" 
@@ -130,172 +75,6 @@ lemma aux':
   apply fri
   done
 
-lemma SomeSup_D: "Some y \<le> Sup {M' a |a. (r, a) \<in> RR} \<Longrightarrow> (\<exists>a. (r, a) \<in> RR)"
-  unfolding Sup_option_def by (auto split: if_splits)
-
-lemma aux_loose:
-  fixes M :: "_ \<rightharpoonup> ecost"
-  assumes "\<And>r. r\<in>dom M \<Longrightarrow> (\<exists>a. (r,a)\<in>RR) \<Longrightarrow> Sup {M' a| a. (r,a)\<in>RR} \<in> {M' a| a. (r,a)\<in>RR}"
-  assumes "SPECT M \<le> \<Down> RR (SPECT M')"
-  shows "\<forall>r\<in>dom M. \<exists>r'. (r,r')\<in>RR \<and> M r \<le> M' r'"
-  using assms
-  (* with single_valued RR *)
-  apply (auto simp: conc_fun_RES)
-  unfolding le_fun_def 
-  subgoal premises p for r y using p(2)[rule_format, of r] p(1)[of r, OF _ SomeSup_D] p(3)
-    by force
-  done
-
-lemma aux_loose':
-  fixes M :: "_ \<rightharpoonup> ecost"
-  assumes "\<And>r. r\<in>dom M \<Longrightarrow> (\<exists>a. (r,a)\<in>RR) \<Longrightarrow> Sup {M' a| a. (r,a)\<in>RR} \<in> {M' a| a. (r,a)\<in>RR}"
-  assumes "SPECT M \<le> \<Down> RR (SPECT M')"
-  assumes "Some cr \<le> M r"
-  shows "\<exists>r'. (r,r')\<in>RR \<and> M r \<le> M' r'"
-  using assms aux_loose[of M RR M']
-  by fastforce
-
-
-lemma single_valued_SupinSup:
-  fixes M' :: "_ \<Rightarrow> (_::complete_lattice) option"
-  shows "single_valued RR \<Longrightarrow> (\<exists>a. (r,a)\<in>RR) \<Longrightarrow> Sup {M' a| a. (r,a)\<in>RR} \<in> {M' a| a. (r,a)\<in>RR}"
-proof -
-  assume SV: "single_valued RR" and "(\<exists>a. (r,a)\<in>RR)"
-  then obtain a where "(r,a)\<in>RR" by auto
-  then have "{M' a| a. (r,a)\<in>RR} = {M' a}"
-    apply auto using SV[THEN single_valuedD] by auto
-  then show ?thesis by auto
-qed
-  
-
-lemma conc_fun_inRR: "SPECT x2 \<le> \<Down> RR (SPECT M) \<Longrightarrow> r \<in> dom x2 \<Longrightarrow> (\<exists>a. (r,a)\<in>RR)"
-  unfolding conc_fun_def apply auto unfolding le_fun_def 
-  subgoal premises p for y apply(rule SomeSup_D)
-    using p(1)[rule_format, of r] p(2) by simp
-  done
-
-lemma domx2:
-  fixes f :: "'d \<Rightarrow> (char list, enat) acost option"
-  shows "Some y \<le> f r \<Longrightarrow> r \<in> dom f"  
-  using ndomIff by fastforce
-
-  
-definition "attains_sup m m' RR \<equiv> 
-  \<forall>r M' M. m=SPECT M \<longrightarrow> m'=SPECT M' \<longrightarrow> r\<in>dom M \<longrightarrow> (\<exists>a. (r,a)\<in>RR) \<longrightarrow> Sup {M' a| a. (r,a)\<in>RR} \<in> {M' a| a. (r,a)\<in>RR}"  
-
-(* Proving attains_sup *)  
-
-(* Single Valued *)
-lemma attains_sup_sv: "single_valued RR \<Longrightarrow> attains_sup m m' RR"  
-  unfolding attains_sup_def
-  using single_valued_SupinSup by fastforce  
-  
-
-(* Tiem does not depend on Result (one-time) *)
- 
-definition "one_time m \<equiv> \<forall>M. m=SPECT M \<longrightarrow> (\<forall>x y s t. M x = Some s \<and> M y = Some t \<longrightarrow> s=t)"
-
-lemma one_time_attains_sup:
-  assumes one_time: "one_time m'"
-  shows "attains_sup m m' RR"
-  unfolding attains_sup_def 
-  apply clarify
-proof -
-  fix r M' M y aa
-  assume [simp]: "m' = SPECT M'" and "(r, aa) \<in> RR"
-  show "\<exists>aa. Sup {M' a |a. (r, a) \<in> RR} = M' aa \<and> (r, aa) \<in> RR" (is "\<exists>_. Sup ?MM = _ \<and> _")
-  proof (cases "\<exists>a c. (r,a)\<in>RR \<and> M' a = Some c")
-    case True
-    then obtain a c where 1: "(r,a)\<in>RR" "M' a = Some c" by blast
-    with one_time have "Some c \<in> ?MM" "?MM \<subseteq> {None,Some c}"
-      unfolding one_time_def
-      by (auto) metis
-    thus ?thesis using 1
-      by (smt Sup_insert Sup_le_iff Sup_subset_mono cSup_eq_maximum ccpo_Sup_singleton empty_Sup insert_commute) 
-  next
-    case False   
-    hence "?MM = {None}" using \<open>(r,aa)\<in>RR\<close> by force
-    thus ?thesis using False \<open>(r,aa)\<in>RR\<close> by auto
-  qed      
-qed  
-
-
-
-lemma OT_return: "one_time (RETURNT x)"
-  unfolding one_time_def by auto
-  
-lemma OT_consume: "one_time m \<Longrightarrow> one_time (consume m c)"  
-  unfolding one_time_def consume_def
-  by (auto split: nrest.splits; blast)
-  
-lemma OT_assert: "one_time (ASSERT \<Phi>)"  
-  unfolding one_time_def 
-  by (cases \<Phi>) auto
-  
-lemma OT_fail: "one_time FAILT"
-  unfolding one_time_def by auto
-
-lemma OT_spec: "one_time (SPEC P (\<lambda>_. c))"
-  unfolding one_time_def SPEC_def by auto
-  
-    
-lemma attains_sup_mop_return:
-  "attains_sup m (do {ASSERT \<Phi>; consume (RETURNT x) (c::ecost)}) R"
-  apply (rule one_time_attains_sup)
-  apply (cases \<Phi>; simp add: OT_consume OT_return OT_fail)
-  done
-
-lemma attains_sup_mop_spec:
-  "attains_sup m (do {ASSERT \<Phi>; SPEC P (\<lambda>_. c::ecost)}) R"
-  apply (rule one_time_attains_sup)
-  apply (cases \<Phi>; simp add: OT_consume OT_return OT_fail OT_spec)
-  done
-
-
-  
-  
-  
-  
-  
-lemma hn_refine_result_loose:
-  assumes R: "hn_refine P c Q R m"
-  assumes LE: "m\<le>\<Down>RR m'"
-  assumes WB: "attains_sup m m' RR"
-  shows "hn_refine P c Q (hr_comp R RR) m'"
-  supply WB' = WB[unfolded attains_sup_def, rule_format]
-  unfolding hn_refine_def
-  apply clarify
-  using LE apply (cases m; simp)
-  apply (frule (1) R[unfolded hn_refine_def, rule_format, rotated], simp)
-  apply (elim exE conjE)
-  subgoal premises p for F s cr M x2 ra Ca
-    using aux_loose'[OF WB'[OF p(4,1)], simplified, OF _ p(3,5), simplified] p(5,6)
-    apply -
-    apply (elim exE conjE)
-
-    apply (intro exI conjI)
-     apply (rule order_trans, assumption+)  
-
-    apply (erule wp_post_cons)
-    unfolding hr_comp_def
-    apply (rule ENTAILSD)
-    apply fri
-    done
-  done
-
-
-lemma hn_refine_result_loose_SV:
-  assumes R: "hn_refine P c Q R m"
-  assumes LE: "m\<le>\<Down>RR m'"
-  assumes SV: "single_valued RR"
-  shows "hn_refine P c Q (hr_comp R RR) m'"
-  apply(rule hn_refine_result_loose)
-    apply fact
-   apply fact
-  apply(rule attains_sup_sv)
-   apply (rule SV)
-  done
-
 
 lemma hn_refine_result:
   assumes R: "hn_refine P c Q R m"
@@ -318,37 +97,9 @@ lemma hn_refine_result:
   apply (rule ENTAILSD)
   apply fri
   done
-    
-lemma hn_refine_cons_res_complete:
-  assumes R: "hn_refine P' c Q R m"
-  assumes I: "P\<turnstile>P'"
-  assumes I': "Q\<turnstile>Q'"
-  assumes R': "\<And>x y. R x y \<turnstile> R' x y"
-  assumes LE: "m\<le>\<Down>RR m'"
-  assumes SV: "single_valued RR"
-  shows "hn_refine P c Q' (hr_comp R RR) m'"
-  apply (rule hn_refine_result)
-  apply (rule hn_refine_cons)
-  by (fact|simp)+
 
-lemma hn_refine_cons_res_complete_loose:
-  assumes R: "hn_refine P' c Q R m"
-  assumes I: "P\<turnstile>P'"
-  assumes I': "Q\<turnstile>Q'"
-  assumes R': "\<And>x y. R x y \<turnstile> R' x y"
-  assumes LE: "m\<le>\<Down>RR m'"
-  assumes AS: "attains_sup m m' RR"
-  shows "hn_refine P c Q' (hr_comp R RR) m'"
-  apply (rule hn_refine_result_loose)
-  apply (rule hn_refine_cons)
-  by (fact|simp)+
-  
-  
-  
-  
-  
-  
-    
+end
+   
 
   abbreviation "raw_array_assn \<equiv> \<upharpoonleft>LLVM_DS_NArray.narray_assn"
 
@@ -384,7 +135,6 @@ lemma lift_acost_plus_distrib[named_ss fri_prepare_simps]:
   apply (auto simp add: sep_algebra_simps fun_eq_iff sep_conj_def sep_disj_acost_def sep_disj_enat_def)
   done
 
-abbreviation "id_assn \<equiv> pure Id"  
 abbreviation "snat_assn \<equiv> \<upharpoonleft>snat.assn"
  
 lemma DECOMP_HNR[vcg_decomp_rules]: "DECOMP_HTRIPLE (hn_refine \<Gamma> c \<Gamma>' R a) \<Longrightarrow> hn_refine \<Gamma> c \<Gamma>' R a" by (simp add: vcg_tag_defs)
@@ -911,5 +661,3 @@ lemma "(xs,xsi)\<in>\<langle>A\<rangle>list_rel \<Longrightarrow> i<length xs \<
     
   
 end
-
-
